Convert to nat64, a transparent dependent type

tools/Vale/test/Semantics.fst
@@ -1,11 +1,26 @@
 module Semantics
 
 open FStar.BaseTypes
-open FStar.UInt64 
-open FStar.Int.Cast
 open FStar.Map
 open FStar.Mul
 
+(* Define some transparently refined int types, 
+   since we only use them in specs, not in emitted code *)
+let nat32_max = 0x100000000
+let nat64_max = 0x10000000000000000
+let _ = assert_norm (pow2 32 = nat32_max)    (* Sanity check our constant *)
+let _ = assert_norm (pow2 64 = nat64_max)    (* Sanity check our constant *)
+
+type nat64 = x:int{0 <= x && x < nat64_max}
+
+(* map type from the F* library, it needs the key type to have decidable equality, not an issue here *)
+type map (key:eqtype) (value:Type) = Map.t key value
+
+(* syntax for map accesses, m.[key] and m.[key] <- value *)
+let op_String_Access     = sel
+let op_String_Assignment = upd
+
+(* Define the operators we support *)
 type reg =
   | Rax
   | Rbx
@@ -29,11 +44,8 @@ type maddr =
   | MReg   : r:reg -> offset:int -> maddr
   | MIndex : base:reg -> scale:int -> index:reg -> offset:int -> maddr
 
-(* REVIEW: Should const be int instead of uint64?  Int gives more flexibility, but 
-           it means that eval_operand has to return int, not uint64.
-           Same question for the regs field in state below *)
 type operand =
-  | OConst: n:uint64 -> operand
+  | OConst: n:nat64 -> operand
   | OReg  : r:reg -> operand
   | OMem  : m:maddr -> operand
 
@@ -75,33 +87,24 @@ type code =
 
 type codes = list code
 
-(* map type from the F* library, it needs the key type to have decidable equality, not an issue here *)
-type map (key:eqtype) (value:Type) = Map.t key value
-
 (* TODO: Eventually this should be a map to bytes.  Simplifying for now *)
-type mem = map int uint64
+type mem = map int nat64
 
 (* state type, noeq qualifier means that this type does not have decidable equality (because of the maps) *)
 noeq type state = {
   ok  :bool;
-  regs:map reg uint64;
-  flags:uint64;
+  regs:map reg nat64;
+  flags:nat64;
   mem :mem;
 }
 
-assume val invalid:uint64
-assume val havoc : state -> ins -> Tot uint64
-
-(* syntax for map accesses, m.[key] and m.[key] <- value *)
-let op_String_Access     = sel
-let op_String_Assignment = upd
+assume val havoc : state -> ins -> Tot nat64
 
 (*
  * writing all the functions as Tot functions
  *)
-
-let eval_reg (r:reg) (s:state) :uint64 =
-  if s.regs `contains` r then s.regs.[r] else invalid
+let eval_reg (r:reg) (s:state) :nat64 =
+  s.regs.[r]
 
 (*
 let valid_resolved_addr (ptr:int) (m:mem) :bool =
@@ -112,18 +115,16 @@ let valid_resolved_addr (ptr:int) (m:mem) :bool =
 *)
 
 (* REVIEW: Is returning invalid the right thing to do here?  Seems like we want !state.ok if this happens *)
-let eval_mem (ptr:int) (s:state) :uint64 =
-  if s.mem `contains` ptr then s.mem.[ptr] else invalid
+let eval_mem (ptr:int) (s:state) :nat64 =
+  s.mem.[ptr]
 
-(* REVIEW: Use FStar.Integers? *)
 let eval_maddr (m:maddr) (s:state) :int =
   match m with
   | MConst n -> n
-  | MReg reg offset -> (FStar.UInt64.v (eval_reg reg s)) + offset
-  | MIndex base scale index offset -> (v (eval_reg base s)) + (scale * (v (eval_reg index s))) + offset
+  | MReg reg offset -> (eval_reg reg s) + offset
+  | MIndex base scale index offset -> eval_reg base s + scale * eval_reg index s + offset
 
-
-let eval_operand (o:operand) (s:state) :uint64 =
+let eval_operand (o:operand) (s:state) :nat64 =
   match o with
   | OConst n -> n
   | OReg r   -> eval_reg r s
@@ -132,45 +133,48 @@ let eval_operand (o:operand) (s:state) :uint64 =
 (* REVIEW: Is it strange to have a dangling v before each term? *)
 let eval_ocmp (s:state) (c:ocmp) :bool =
   match c with
-  | OEq o1 o2 -> v (eval_operand o1 s) = v (eval_operand o2 s)
-  | ONe o1 o2 -> v (eval_operand o1 s) <> v (eval_operand o2 s)
-  | OLe o1 o2 -> v (eval_operand o1 s) <= v (eval_operand o2 s)
-  | OGe o1 o2 -> v (eval_operand o1 s) >= v (eval_operand o2 s)
-  | OLt o1 o2 -> v (eval_operand o1 s) < v (eval_operand o2 s)
-  | OGt o1 o2 -> v (eval_operand o1 s) > v (eval_operand o2 s)
+  | OEq o1 o2 -> eval_operand o1 s = eval_operand o2 s
+  | ONe o1 o2 -> eval_operand o1 s <> eval_operand o2 s
+  | OLe o1 o2 -> eval_operand o1 s <= eval_operand o2 s
+  | OGe o1 o2 -> eval_operand o1 s >= eval_operand o2 s
+  | OLt o1 o2 -> eval_operand o1 s < eval_operand o2 s
+  | OGt o1 o2 -> eval_operand o1 s > eval_operand o2 s
 
-let update_reg (r:reg) (s:state) (v:uint64) :state = { s with regs = s.regs.[r] <- v }
+let update_reg (r:reg) (s:state) (v:nat64) :state = { s with regs = s.regs.[r] <- v }
 
-let update_mem (ptr:int) (s:state) (v:uint64) :state = { s with mem = s.mem.[ptr] <- v }
+let update_mem (ptr:int) (s:state) (v:nat64) :state = { s with mem = s.mem.[ptr] <- v }
 
-let update_operand (o:dst_op) (s:state) (v:uint64) :state =
+let update_operand (o:dst_op) (s:state) (v:nat64) :state =
   match o with
   | OReg r   -> update_reg r s v
   | OMem m   -> update_mem (eval_maddr m s) s v
 
-let update_operand_and_flags (o:dst_op) (s:state) (ins:ins) (v:uint64) :state =
+let update_operand_and_flags (o:dst_op) (s:state) (ins:ins) (v:nat64) :state =
   { (update_operand o s v) with flags = havoc s ins }
 
-(* REVIEW: Is there a cleaner way to write this? *)
-let cf (flags:uint64) :bool =
-  v (logand flags 1uL) > 0
+(* REVIEW: Will we regret exposing a mod here?  Should flags be something with more structure? *)
+let cf (flags:nat64) :bool =
+  flags % 2 = 1
 
-let update_cf (flags:uint64) (cf:bool) :uint64 =
-  if cf then logor flags 1uL
-  else flags
-
-let uint32_max = 0x100000000
-let uint64_max = 0x10000000000000000
-let _ = assert_norm (pow2 32 = uint32_max)    (* Sanity check our constant *)
-let _ = assert_norm (pow2 64 = uint64_max)    (* Sanity check our constant *)
+let update_cf (flags:nat64) (new_cf:bool) :nat64 =
+  if new_cf then
+    if not (cf flags) then
+      flags + 1
+    else
+      flags
+  else 
+    if (cf flags) then
+      flags - 1
+    else
+      flags
 
 (* REVIEW: What's the best way to handle "valid shift amount" for shift instructions?  It depends on ins and state.
            Approach below makes the machine go bad if you use an invalid amount
  *)
 let valid_shift_operand (o:operand) (s:state) :bool =
-  (OConst? o && 0 <= v (OConst?.n o) && v (OConst?.n o) < 32) 
+  (OConst? o && 0 <= OConst?.n o && OConst?.n o < 32) 
   || 
-  ((OReg? o) && (Rcx? (OReg?.r o)) && v (eval_operand o s) < uint32_max)
+  ((OReg? o) && (Rcx? (OReg?.r o)) && eval_operand o s < nat32_max)
 
 #reset-options "--z3rlimit 100"
 let eval_ins (ins:ins) (s:state) :state =
@@ -178,25 +182,25 @@ let eval_ins (ins:ins) (s:state) :state =
   else
     match ins with 
     | Mov64 dst src -> update_operand dst s (eval_operand src s)
-    | Add64 dst src -> update_operand_and_flags dst s ins (eval_operand dst s +%^ eval_operand src s)
-    | AddLea64 dst src1 src2 -> update_operand_and_flags dst s ins (eval_operand src1 s +%^ eval_operand src2 s)
+    | Add64 dst src -> update_operand_and_flags dst s ins ((eval_operand dst s + eval_operand src s) % nat64_max)
+    | AddLea64 dst src1 src2 -> update_operand_and_flags dst s ins ((eval_operand src1 s + eval_operand src2 s) % nat64_max)
     | AddCarry64 dst src -> let old_carry = if cf(s.flags) then 1 else 0 in
-			   let sum = v (eval_operand dst s) + v (eval_operand src s) + old_carry in			  
-			   let new_carry = sum > uint64_max in
-			   { update_operand dst s (uint_to_t (sum % uint64_max)) with flags = update_cf s.flags new_carry }
-    | Sub64 dst src -> update_operand_and_flags dst s ins (eval_operand dst s -%^ eval_operand src s)
-    | Mul64 src -> let product = v (eval_reg Rax s) * v (eval_operand src s) in
-		  let hi = uint_to_t (product / uint64_max) in
-		  let lo = uint_to_t (product % uint64_max) in
+			   let sum = eval_operand dst s + eval_operand src s + old_carry in			  
+			   let new_carry = sum > nat64_max in
+			   { update_operand dst s (sum % nat64_max) with flags = update_cf s.flags new_carry }
+    | Sub64 dst src -> update_operand_and_flags dst s ins ((eval_operand dst s - eval_operand src s) % nat64_max)
+    | Mul64 src -> let product = eval_reg Rax s * eval_operand src s in
+		  let hi = product / nat64_max in
+		  let lo = product % nat64_max in
 		  { update_reg Rax (update_reg Rdx s hi) lo with flags = havoc s ins }
-    | IMul64 dst src -> update_operand_and_flags dst s ins (eval_operand dst s *%^ eval_operand src s)	  
-    | Xor64 dst src -> update_operand_and_flags dst s ins (eval_operand dst s ^^ eval_operand src s)	  
+    | IMul64 dst src -> update_operand_and_flags dst s ins ((eval_operand dst s * eval_operand src s) % nat64_max)	  
+    | Xor64 dst src -> update_operand_and_flags dst s ins (FStar.Int.logxor #64 (eval_operand dst s) (eval_operand src s))	  
     | Shr64 dst amt -> if valid_shift_operand amt s then			
-		        update_operand_and_flags dst s ins (shift_right (eval_operand dst s) (uint64_to_uint32 (eval_operand amt s)))
+		        update_operand_and_flags dst s ins (FStar.Int.shift_right #64 (eval_operand dst s) (eval_operand amt s))
 		      else
 			{ s with ok = false }
     | Shl64 dst amt -> if valid_shift_operand amt s then			
-		        update_operand_and_flags dst s ins (shift_left (eval_operand dst s) (uint64_to_uint32 (eval_operand amt s)))
+		        update_operand_and_flags dst s ins (FStar.Int.shift_left #64 (eval_operand dst s) (eval_operand amt s))
 		      else
 			{ s with ok = false }
 
@@ -207,7 +211,7 @@ let eval_ins (ins:ins) (s:state) :state =
 let decr (c:code) (s:state) :nat =
   match c with
   | While _ _ inv ->
-    let n = v (eval_operand inv s) in
+    let n = eval_operand inv s in
     if n >= 0 then n else 0
   | _             -> 0
 
@@ -236,7 +240,7 @@ and eval_codes l s =
     
 and eval_while c s_0 = (* trying to mimic the eval_while predicate using a function *)
   let While cond body inv = c in
-  let n_0 = v (eval_operand inv s_0) in
+  let n_0 = eval_operand inv s_0 in
   let b = eval_ocmp s_0 cond in
 
   if n_0 <= 0 then
@@ -250,6 +254,6 @@ and eval_while c s_0 = (* trying to mimic the eval_while predicate using a funct
         let s_1 = Some?.v s_opt in
 	if not s_1.ok then Some s_1  //this is from the reference semantics, if ok flag is unset, return
 	else
-	  let n_1 = v (eval_operand inv s_1) in
+	  let n_1 = eval_operand inv s_1 in
 	  if n_1 >= n_0 then None  //loop invariant must decrease
 	  else eval_while c s_1
